

Subject _____

AVD611-Modern Signal Processing Tutorial-3

①

$$H(z) = \frac{1 - 0.5z^{-1}}{1 - 0.75z^{-1}}$$

$$r_x(k) = (1/3)^{|k|}$$

$$\Rightarrow P_x(z) = \sum_{m=-\infty}^{\infty} (1/3)^{|m|} z^{-m}$$

$$= \sum_{m=-\infty}^{-1} (1/3)^{-m} z^{-m} + \sum_{m=0}^{\infty} (1/3)^m z^{-m}$$

$$= \frac{1}{1 - az^{-1}} + \frac{1}{1 - az^{-1}}$$

$$= \frac{1 - a^2}{1 - a(z + z^{-1}) + a^2}, \quad a = 1/3$$

\therefore Output power spectrum,

$$P_y(z) = H(z) H^*(z^{-1}) P_x(z)$$

$$= \frac{1 - 0.5z^{-1}}{1 - 0.75z^{-1}} \cdot \frac{1 - 0.5z}{1 - 0.75z} \cdot \frac{1 - (1/3)^2}{1 - \frac{1}{3}(z + z^{-1}) + (\frac{1}{3})^2}$$

$$= \frac{1.25 - 0.5(z + z^{-1})}{1.5625 - 0.75(z + z^{-1})} \cdot \frac{8/9}{1 - \frac{1}{3}(z + z^{-1}) + \frac{1}{9}}$$

$$= \frac{8}{9} \frac{1.25 - 0.5(z + z^{-1})}{1.5625 - 0.75(z + z^{-1})} \cdot \frac{1}{\frac{10}{9} - \frac{1}{3}(z + z^{-1})}$$

$$= \frac{8 [1.25 - 0.5(z + z^{-1})]}{1.5625 - 0.75(z + z^{-1})} \cdot \frac{1}{10 - 3(z + z^{-1})}$$

Now, $P_y(z) = \frac{8}{9} \frac{[1.25 - 0.5(z + z^{-1})]}{(1 - 0.75z^{-1})(1 - 0.75z)(1 - \frac{1}{3}z^{-1})(1 - \frac{1}{3}z)}$

$$\downarrow \text{IZT} = \frac{2/3}{(1 - 0.75z^{-1})(1 - 0.75z)} + \frac{2/9}{(1 - \frac{1}{3}z^{-1})(1 - \frac{1}{3}z)}$$

$$\Rightarrow r_y(k) = \frac{2}{3} (0.75)^{|k|} + \frac{2}{9} \left(\frac{1}{3}\right)^{|k|}$$

$$= \begin{cases} \frac{4}{3} (0.75)^k - \frac{4}{9} \left(\frac{1}{3}\right)^k, & k \geq 0 \\ \frac{4}{3} \left(\frac{1}{3}\right)^{-k} - \frac{4}{9} \left(\frac{1}{3}\right)^{-k}, & k < 0 \end{cases}$$

② ① $y_x(k) = \delta(k) + 2(0.5)^{|k|}$

$$\begin{aligned} ZT \Rightarrow P_X(Z) &= 1 + 2 \left[\frac{1 - (0.5)^2}{1 - 0.5(Z + Z^{-1}) + 0.5^2} \right] \\ &= 1 + \frac{2(0.75)}{1.25 - 0.5(Z + Z^{-1})} \end{aligned}$$

⑦ $x_k(k) = \begin{cases} 10 - |k|, & |k| < 10 \\ 0, & \text{otherwise} \end{cases}$

↓
 triangular → convolution of two rectangular sequences
 Triangular autocorrelation → autocorr. of rectangular sequence

$\therefore P_X(e^{j\omega}) = |W(e^{j\omega})|^2$, $W(e^{j\omega})$ being DTFT of some $w(n)$ sequence.

$$W(e^{j\omega}) = \sum_{n=0}^{N-1} e^{j\omega n} = e^{j\omega(N-1)/2} \frac{\sin(N\omega/2)}{\sin(\omega/2)}$$

$$\Rightarrow |W(e^{j\omega})|^2 = \left| \frac{\sin(N\omega/2)}{\sin(\omega/2)} \right|^2$$

For $N=10$,

$$P_x(e^{j\omega}) = \left| \frac{\sin(10\omega/2)}{\sin(\omega/2)} \right|^2$$

③

$$P_x(z) = \frac{-2z^2 + 5z - 2}{3z^2 + 10z + 3}$$

$$= \frac{\cancel{z^2} - 2 + 5\cancel{z} - 2z^{-2}}{3 + 10z^{-1} + 3z^{-2}}$$

$$= \frac{-2 + 5z^{-1} - 2z^{-2}}{(1+3z^{-1})(3+z^{-1})}$$

$$= \frac{-\frac{1}{2} + \frac{1}{2}z^{-1}}{1+3z^{-1}} + \frac{-\frac{1}{2} - \frac{1}{2}z^{-1}}{3+z^{-1}}$$

$$= \frac{-1}{2} \frac{1-z^{-1}}{1+3z^{-1}} + \frac{-1}{2} \frac{1+z^{-1}}{3+z^{-1}}$$

$$\Rightarrow y_x(k) = \frac{-1}{2} \left[(-3)^k u(k) - (-3)^{k-1} u(k-1) + \left(-\frac{1}{3}\right)^k u(k) + \left(-\frac{1}{3}\right)^{k-1} u(k-1) \right]$$

④

$$x(k) = 10\left(\frac{1}{2}\right)^{|k|} + 3\left(\frac{1}{2}\right)^{|k-1|} + 3\left(\frac{1}{2}\right)^{|k+1|}$$

$$y(k) = \delta(k) \quad [\text{white}]$$

$$P_x(z) = 10 \left[\frac{1 - \frac{1}{4}}{1 - \frac{1}{2}(z+z^{-1}) + \frac{1}{4}} \right] + \frac{3z^{-1} \left(\frac{3}{4}\right)}{\frac{5}{4} - \frac{1}{2}(z+z^{-1})} + \frac{3z \left(\frac{3}{4}\right)}{\frac{5}{4} - \frac{1}{2}(z+z^{-1})}$$

$$= \frac{10 + 3(z+z^{-1})}{\frac{5}{4} - \frac{1}{2}(z+z^{-1})}$$

$$= \frac{\frac{3}{4}(10z + 3z^2 + 3)}{1.25z - \frac{1}{2}(z^2 + 1)}$$

$$= \frac{-3}{2} \frac{3z^2 + 10z + 3}{z^2 - 2.5z + 1}$$

[Multiply N^r & D^r by z]

$$= K \frac{(3z^2 + 10z + 3)}{(z+2)(z+1/2)} \quad (K > 0)$$

$$= A(z) A(z^{-1}), \text{ where } A(z) = \sqrt{K} \frac{3z+1}{z-1/2}$$

∴ Whitening filter $[y(n) = h_w(n) * x(n)]$,

$$H_w(z) = \frac{1}{A(z)}$$

$$= \frac{(z-1/2)}{\sqrt{K}(3z+1)}$$

$$\text{choose } K=1 \Rightarrow H_w(z) = \frac{z-1/2}{3z+1}$$

(o/p variance = 1)

⑤ $x(n) = 4v(n) - 2v(n-1) + v(n-2), \quad \sigma_v^2 = 1$

$$r_x(k) = E[x(n)x(n+k)]$$

$$\Rightarrow r_x(0) = E[x^2(n)] = E[(4v(n) - 2v(n-1) + v(n-2))^2]$$

$$= \sigma_v^2(16 + 4 + 1)$$

$$= 21\sigma_v^2 = 21$$

$$r_x(1) = E[x(n)x(n+1)]$$

$$= \sigma_v^2[4(-2) + (-2)(1)] = -10$$

$$r_x(2) = 4\sigma_v^2 = 4, \quad r_x(3) = 0$$

$$\text{Now, } \begin{bmatrix} r_x(0) & r_x(1) \\ r_x(1) & r_x(0) \end{bmatrix} \begin{bmatrix} h_1 \\ h_2 \end{bmatrix} = \begin{bmatrix} r_x(2) \\ r_x(3) \end{bmatrix}$$

$$\Rightarrow \begin{pmatrix} 21 & -10 \\ -10 & 21 \end{pmatrix} \begin{pmatrix} h_1 \\ h_2 \end{pmatrix} = \begin{pmatrix} 4 \\ 0 \end{pmatrix}$$

$$\Rightarrow 21h_1 - 10h_2 = 4,$$

$$-10h_1 + 21h_2 = 0 \Rightarrow h_1 = 21/10 h_2$$

$$\Rightarrow h_1 = \frac{84}{341}, \quad h_2 = \frac{40}{341}$$

$$\text{MMSE} = r_x(0) - [r_x(2) - r_x(3)] \begin{bmatrix} r_x(0) & r_x(1) \\ r_x(1) & r_x(0) \end{bmatrix}^{-1} \begin{bmatrix} r_x(2) \\ r_x(3) \end{bmatrix}$$

$$\begin{aligned}
 &= 21 - \begin{bmatrix} 4 & 0 \end{bmatrix} \begin{bmatrix} 21 & -10 \\ -10 & 21 \end{bmatrix}^{-1} \begin{bmatrix} 4 \\ 0 \end{bmatrix} \\
 &= 21 - \begin{bmatrix} 4 & 0 \end{bmatrix} \frac{1}{341} \begin{pmatrix} 21 & 10 \\ 10 & 21 \end{pmatrix} \begin{pmatrix} 4 \\ 0 \end{pmatrix} \\
 &= 21 - \frac{1}{341} (4 \ 0) \begin{pmatrix} 84 \\ 40 \end{pmatrix} \\
 &= 21 - \frac{1}{341} \times 336 = \frac{6825}{341} \approx 20.01.
 \end{aligned}$$

⑥ @ $y(n) = x(n) + 0.8x(n-1) + v(n)$, $\sigma_v^2 = 1$

$$r_x = [4 \ 2 \ 1 \ 0.5]^T$$

$$= 4(0.5)^{|k|}$$

$$\begin{aligned}
 \Rightarrow P_x(z) &= 4 \frac{(1-0.25)}{1 - \frac{1}{2}(z+z^{-1}) + \frac{1}{4}} \\
 &= \frac{3}{1.25 - 0.5(z+z^{-1})}
 \end{aligned}$$

Also, $y(z) = x(z) + 0.8z^{-1}x(z) + \cancel{v(z)}^1 = (1+0.8z^{-1})x(z) + 1$

$$H(z) = \frac{P_{xy}(z)}{P_y(z)} = \frac{P_x(z)}{P_y(z)}$$

$$\begin{aligned}
 &= \frac{3}{1.25 - 0.5(z+z^{-1})} \cdot \frac{1}{[(1+0.8z^{-1})]^2 P_x(z) + 1} \\
 &= \frac{3}{1.25 - 0.5(z+z^{-1})} \cdot \frac{1}{8(1+0.8z^{-1})(1+0.8z) + 1} \\
 &= \frac{1.25 - 0.5(z+z^{-1})}{(1+0.8z^{-1})(1+0.8z) + 1.25 - 0.5(z+z^{-1})} \\
 &= \frac{1.25 - 0.5(z+z^{-1})}{1.64 + 0.8(z+z^{-1}) + 1.25 - 0.5(z+z^{-1})} \\
 &= \frac{1.25 - 0.5(z+z^{-1})}{2.89 - 0.3(z+z^{-1})}
 \end{aligned}$$

$$\begin{aligned}
 \textcircled{6} \quad H(z) &= \frac{1.25z - 0.5z^2 - 0.5}{0.89z - 0.3z^2 - 0.3} \\
 &= \frac{0.5z^2 - 1.25z + 0.5}{0.3z^2 - 0.89z + 0.3} \\
 &= \frac{0.5(z-2)(z-1/2)}{0.3(z-0.1)(z-9.5)} \\
 &= \frac{5/3}{(1-0.1z^{-1})(1-9.5z^{-1})} \frac{(1-2z^{-1})(1-1/2z^{-1})}{(1-0.1z^{-1})(1-9.5z^{-1})}
 \end{aligned}$$

$$H_{\text{causal}}(z) = \frac{5}{3} \frac{(1-1/2z^{-1})(1-2z^{-1})}{(1-0.1z^{-1})}$$

$$\textcircled{7} \quad x(n) = x(n-1) - 0.6x(n-2) + w(n), \quad \sigma_w^2$$

Yule Walker eqn:

$$\begin{pmatrix} r_x(0) & r_x(1) & r_x(2) \\ r_x(1) & r_x(0) & r_x(1) \\ r_x(2) & r_x(1) & r_x(0) \end{pmatrix} \begin{pmatrix} 1 \\ -1 \\ 0.6 \end{pmatrix} = \begin{pmatrix} \sigma_w^2 \\ 0 \\ 0 \end{pmatrix}$$

$$\Rightarrow r_x(0) - r_x(1) + 0.6 r_x(2) = \sigma_w^2$$

$$r_x(1) - r_x(0) + 0.6 r_x(1) = 0 \Rightarrow 1.6 r_x(1) = r_x(0)$$

$$r_x(2) - r_x(1) + 0.6 r_x(0) = 0 \Rightarrow r_x(2) = 0.04 r_x(1)$$

$$\Rightarrow 1.6 r_x(1) - r_x(1) + 0.024 r_x(1) = \sigma_w^2$$

$$\Rightarrow 0.624 r_x(1) = \sigma_w^2$$

$$\Rightarrow r_x(1) = 1.60 \sigma_w^2$$

$$r_x(0) = 2.56 \sigma_w^2$$

$$r_x(2) = 0.064 \sigma_w^2$$

$$\textcircled{8} \quad x(n) = s(n) + w(n)$$

$$s(n) = 0.4 s(n-1) + v(n), \quad \sigma_w^2 = 1, \sigma_v^2 = 0.49$$

$$\textcircled{a} \quad r_s(m) = E[s(n)s(n+m)]$$

$$= E[\{0.4s(n-1) + v(n)\} \{0.4s(n+m-1) + v(n+m)\}]$$

$$= 0.16 r_s(m) + r_v(m)$$

$$\Rightarrow 0.84 r_s(m) = r_v(m)$$

$$\begin{aligned}\Rightarrow r_s(m) &= 1.19 r_v(m) \\ &= 1.19 \times 0.49 \delta(m) \\ &= 0.58 \delta(m).\end{aligned}$$

$$\begin{aligned}\text{Also, } r_x(m) &= r_s(m) + r_w(m) \\ &= 0.58 \delta(m) + \delta(m) \\ &= 1.58 \delta(m).\end{aligned}$$

⑥ Wiener filter, $h = R_x^{-1} r_{sx}$

$$\begin{aligned}\begin{pmatrix} h_0 \\ h_1 \end{pmatrix} &= \begin{pmatrix} r_x(0) & r_x(1) \\ r_x(1) & r_x(0) \end{pmatrix} \begin{pmatrix} r_{sx}(0) \\ r_{sx}(1) \end{pmatrix} \\ &= \begin{pmatrix} 0.58 & 0 \\ 0 & 1.58 \end{pmatrix} \begin{pmatrix} 0.58 \\ 0 \end{pmatrix} \\ &= \begin{pmatrix} 0.916 \\ 0 \end{pmatrix}\end{aligned}$$

⑦ MMSE = $r_s(0) - \begin{bmatrix} r_{sx}(0) & r_{sx}(1) \end{bmatrix} \begin{bmatrix} r_x(0) & r_x(1) \\ r_x(1) & r_x(0) \end{bmatrix}^{-1} \begin{pmatrix} r_{xs}(0) \\ r_{xs}(1) \end{pmatrix}$

$$\begin{aligned}&= 0.58 - \begin{bmatrix} 0.58 & 0 \end{bmatrix} \begin{bmatrix} 1.58 & 0 \\ 0 & 1.58 \end{bmatrix}^{-1} \begin{bmatrix} 0.58 \\ 0 \end{bmatrix} \\ &= 0.58 - \begin{bmatrix} 0.58 & 0 \end{bmatrix} \frac{1}{2.49} \begin{bmatrix} 1.58 & 0 \\ 0 & 1.58 \end{bmatrix} \begin{bmatrix} 0.58 \\ 0 \end{bmatrix} \\ &= 0.58 - \frac{1}{2.49} \begin{bmatrix} 0.58 & 0 \end{bmatrix} \begin{bmatrix} 0.916 \\ 0 \end{bmatrix} \\ &= 0.58 - \frac{1}{2.49} \begin{bmatrix} 0.531 \\ 0 \end{bmatrix} \\ &= 0.366\end{aligned}$$